randRangeNonZero(-10, 10) randRangeNonZero(-10, 10) randRangeNonZero(-10, 10) randRangeNonZero(-5, 5) randRangeNonZero(-5, 5) rand(2)

Evaluate the following expression.

A + (B \times negParens(C)) A + B \times negParens(C)

A + B * C

= A + (B * C)

= A + B * C

= A + B * C

A \times (B + negParens(C))

A * (B + C)

= A \times B + C

= A * (B + C)

A + \left(\dfrac{B * C}{C}\right) A + \dfrac{B * C}{C}

A + B

= A + (B)

= A + B

= A + B

\dfrac{A * (B + C)}{B + C}

A

= \dfrac{A * (B + C)}{B + C }

= A

(A + (B - C \times negParens(D))) \times negParens(E)

(A + (B - (C * D))) * E

= (A + (B - C * D)) \times negParens(E)

= (A + (B - (C * D))) \times negParens(E)

= (A + B - (C * D)) \times negParens(E)

= (A + (B - (C * D))) \times negParens(E)

= A + (B - (C * D)) \times negParens(E)

= (A + (B - (C * D))) * E

A + (B + C \times negParens(D)) \times negParens(E)

A + ((B + (C * D)) * E)

= A + (B + C * D) \times negParens(E)

= A + (B + C * D) \times negParens(E)

= A + (B + C * D) * E

= A + (B + C * D) * E

A + B \times negParens(C) + \dfrac{(D * E)}{E}

A + B * C + D

= A + B \times negParens(C) + D

= A + B * C + D

= A + B * C + D

= A + B * C + D

A \times negParens(B) + C \times \dfrac{(D * E)}{E}

(A * B) + (C * D)

= A \times negParens(B) + C \times negParens(D)

= A * B + C \times negParens(D)

= A * B + C * D

= A * B + C * D

(A + B \times negParens(D)) - C \times negParens(E) A + B \times negParens(D) - C \times negParens(E)

A + B * D - C * E

= (A + B * D) - C \times negParens(E)

= A + B * D - C \times negParens(E)

= A + B * D - C * E

= A + B * D - C * E

= A + B * D - C * E

A - negParens(B)^2

A - B * B

= A - B * B

= A - B * B

randRangeNonZero(-10, 10) randRangeNonZero(-10, 10)

A - (B + C)^2

A - (B + C) * (B + C)

= A - (B + C)^2

= A - (B + C) * (B + C)

= A - (B + C) * (B + C)